$$\begin{array}{ccc}
x^{1} \equiv x \mod P(x) & x^{2} \equiv x^2 \mod P(x) & x^{3} \equiv x^2 - 1 \mod P(x) \\
x^{4} \equiv x^2 - x - 1 \mod P(x) & x^{5} \equiv - x - 1 \mod P(x) & x^{6} \equiv - x^2 - x \mod P(x) \\
x^{7} \equiv x^2 + 1 \mod P(x) & x^{8} \equiv x^2 + x - 1 \mod P(x) & x^{9} \equiv - x^2 - x - 1 \mod P(x) \\
x^{10} \equiv x^2 - x + 1 \mod P(x) & x^{11} \equiv x - 1 \mod P(x) & x^{12} \equiv x^2 - x \mod P(x) \\
x^{13} \equiv -1 \mod P(x) & x^{14} \equiv - x \mod P(x) & x^{15} \equiv - x^2 \mod P(x) \\
x^{16} \equiv - x^2 + 1 \mod P(x) & x^{17} \equiv - x^2 + x + 1 \mod P(x) & x^{18} \equiv x + 1 \mod P(x) \\
x^{19} \equiv x^2 + x \mod P(x) & x^{20} \equiv - x^2 - 1 \mod P(x) & x^{21} \equiv - x^2 - x + 1 \mod P(x) \\
x^{22} \equiv x^2 + x + 1 \mod P(x) & x^{23} \equiv - x^2 + x - 1 \mod P(x) & x^{24} \equiv - x + 1 \mod P(x) \\
x^{25} \equiv - x^2 + x \mod P(x) & x^{26} \equiv 1 \mod P(x) & \end{array}$$
