\documentclass{article}
\usepackage{enumerate}
\usepackage{amsmath}
\usepackage{amssymb}
\usepackage{graphicx}
\usepackage{subfigure}
\usepackage{geometry}
\usepackage{caption}
\usepackage{indentfirst}
\usepackage{multirow}
\geometry{left=3.0cm,right=3.0cm,top=3.0cm,bottom=4.0cm}
\renewcommand{\thesection}{Ex. \arabic{section} ---}
\renewcommand{\mod}{{\rm\ mod\ }}
\title{VE475 Homework 4}
\author{Liu Yihao 515370910207}
\date{}

\begin{document}
\maketitle

\section{Euler's totient}
\begin{enumerate}
\item 
Suppose $$\varphi(p^k)=p^{k-1}(p-1)=p^k-p^{k-1}$$ which means, there are $p^{k-1}$ integers of $n\in[1,p^k]$ so that $$\gcd(n,p^k)>1$$
What's more, if an integer and $p^k$ is not coprime, it can be divided by $p$ since all of prime factors of $p^k$ are $p$.

When $k=1$, we know $\varphi(p)=p-1$ since $p$ is a prime.

When $k=i$, suppose $\varphi(p^i)=p^{i}-p^{i-1}$.

When $k=i+1$, we know that there are $p^{i-1}$ integers in $[1,p^i]$ which are not coprime with $p^i$, so they are also not coprime with $p^{i+1}$. Then consider the integers $n\in[p^i+1,p^{i+1}]$ which are not coprime with $p^{i+1}$, we know that they all have a prime factor $p$, and $n/p\in[p^{i-1}+1,p^i]$, so there are $(p-1)p^{i-1}$ integers that satisfy this condition. In total, there are $p^{i-1}+(p-1)p^{i-1}=p^{i}$ integers which are not coprime with $p^{i+1}$, so $\varphi(p^{i+1})=p^{i+1}-p^i$.

According to the mathematical induction above, we can concluded that $$\varphi(p^k)=p^{k-1}(p-1)$$

\item
According to the Chinese Reminder Theorem, since $m$ and $n$ are coprime, there exists a ring isomorphism between $Z/mnZ$ and $Z/mZ\times Z/nZ$, and here $\varphi(mn)$ is the order of $Z/mnZ$, $\varphi(m)$ is the order of $Z/mZ$ and $\varphi(n)$ is the order of $Z/nZ$. Suppose $MN$ is the set of counted integers in $\varphi(mn)$, $M$ is that in $\varphi(M)$ and $N$ is that in $\varphi(N)$, there is a bijection between $MN$ and $M\times N$. So $\varphi(mn)=\varphi(m)\varphi(n)$.

\item
Suppose $$n=p_1^{k_1}p_2^{k_2}\cdots p_n^{k_n}$$ where $p_1,p_2,\cdots,p_n$ are primes and $k_1,k_2,\cdots,k_n\geqslant1$, it is obvious that $p_1^{k_1},p_2^{k_2},\cdots,p_n^{k_n}$ are pairwise coprime, so 
\begin{align*}
\varphi(n)&=\varphi(p_1^{k_1})\varphi(p_n^{k_n})\cdots\varphi(p_n^{k_n})\\
&=p_1^{k_1-1}(p_1-1)p_2^{k_2-1}(p_2-1)\cdots p_n^{k_n-1}(p_n-1)\\
&=p_1^{k_1}\left(1-\frac{1}{p_1}\right)p_2^{k_2}\left(1-\frac{1}{p_2}\right)\cdots p_n^{k_n}\left(1-\frac{1}{p_n}\right)\\
&=n\prod_{p|n}\left(1-\frac{1}{p}\right)
\end{align*}

\item
$$\varphi(1000)=1000\left(1-\frac{1}{2}\right)\left(1-\frac{1}{5}\right)=400$$

According to Euler's Theorem, since 7 is coprime with 1000, $$7^{400}\equiv1\mod1000$$
\begin{align*}
7^{803}&\equiv7^3\mod1000\\
&\equiv343\mod1000
\end{align*}
\end{enumerate}

\section{AES}
\begin{enumerate}
\item
128 bits of 1 is used as the key for round 1.
\item
$$K(5)=K(4)\oplus K(1)$$
\item
We know for a 4 bit number $X$, $$X\oplus 1111=\overline{X}$$
We also know $$K(0)=K(1)=K(2)=K(3)=1111$$
So it's easy to find
\begin{align*}
K(10)&=K(9)\oplus K(6)\\
&=[K(8)\oplus K(5)]\oplus[K(5)\oplus K(2)]\\
&=K(8)\oplus K(2)\\
&=\overline{K(8)}\\
K(11)&=K(10)\oplus K(7)\\
&=[K(9)\oplus K(6)]\oplus[K(6)\oplus K(3)]\\
&=K(9)\oplus K(3)\\
&=\overline{K(9)}
\end{align*}
\end{enumerate}

\section{Simple Questions}
\begin{enumerate}
\item
In ECB Mode, each block is encrypted separately with a function $E$ and a key $K$, so the corruption of one encrypted block won't influence other blocks, only one block will be decrypted incorrectly.

In CBC Mode, from the second block, each block is encrypted and xor with the previous encrypted block. If one encrypted block (not the last block) is corrupted, the next block will also be influenced when applied xor with the wrong block, so two blocks will be decrypted incorrectly.

\item
If IV is incremented by 1 each time, after a reset, the attacker would know the exact value of IV every time and can construct whatever plaintext he want and xor it with IV, and then input it into the block cipher. Then he can compare the ciphertext with the plaintext more efficiently. So it is not CPA secure.

\item
Since $p=29$ is a prime, according to Theorem 2.17, we can test the prime factors of $p-1=28$, which are 2 and 7. 

First, when $q=2$, $$2^{(p-1)/q}=2^{28/2}=2^{14}\equiv28\mod 29$$
Second, when $q=7$, $$2^{(p-1)/q}=2^{28/7}=2^{4}\equiv16\mod 29$$
So $$2^{(p-1)/d}\not\equiv1\mod p$$
We can concluded that 2 is a generator of $U(Z/29Z)$.

\item
Since 1801 and 8191 are primes, it is a Legendre Symbol, and we can directly calculate $1801^{4095}\mod8191$ to solve it.

By applying modular exponentiation, we get the following table.
\begin{center}
\begin{tabular}{ccc}
$i$ & $d_i$ & power mod 8191 \\\hline
\input{ex3/4}
\end{tabular}
\end{center}
$$1801^{4095}\equiv8190\mod8191$$
$$\left(\frac{1801}{8191}\right)=-1$$

\item
First, if $\left(\frac{b^2-4ac}{p}\right)=0$, then $b^2-4ac=0$, so the equation only have one solution $x=-\frac{b}{2a}$, and it can always mod $p$, thus the number of solutions satisfies $1+\left(\frac{b^2-4ac}{p}\right)=1$.

Second, if $\left(\frac{b^2-4ac}{p}\right)\neq0$, then $b^2-4ac\neq0$, the equation have two solutions $x=-\frac{b\pm\sqrt{b^2-4ac}}{2a}$, which means
$$-\frac{b\pm\sqrt{b^2-4ac}}{2a}\equiv x\mod p$$
$$\sqrt{b^2-4ac}\equiv \pm(2ax+b)\mod p$$
Then the problem becomes whether $b^2-4ac$ is a square mod $p$.

If $\left(\frac{b^2-4ac}{p}\right)=1$, $b^2-4ac$ is a square mod $p$, and we can get 2 solutions mod $p$.

Otherwise, $\left(\frac{b^2-4ac}{p}\right)=-1$, $b^2-4ac$ is not a square mod $p$, and we can get no solution mod $p$.

In conclusion, the number of solutions mod $p$ to the equation $ax^2+bx+c$ is 
$$1+\left(\frac{b^2-4ac}{p}\right)$$
\item
According to Euler's theorem, $$n^{p-1}\equiv1\mod p$$ $$n^{q-1}\equiv1\mod q$$
Let $(p-1)=k(q-1)$,
$$(n^{q-1})^p=n^{p-1}\equiv1\mod q$$
Since $\gcd(n,pq)=1$, according to Chinese Reminder Theorem, we get
$$n^{p-1}\equiv1\mod pq$$

\item
\begin{enumerate}[(a)]
\item Necessity: We know 
$$\left(\frac{-3}{p}\right)=\left(\frac{-1}{p}\right)\left(\frac{3}{p}\right)=1$$
First, if $p\equiv1\mod4$, $\left(\frac{-1}{p}\right)=1$, then $\left(\frac{3}{p}\right)=1$. And since $p\not\equiv3\mod4$, $\left(\frac{3}{p}\right)=\left(\frac{p}{3}\right)=1$, so $p\equiv1\mod3$, thus $$p\equiv1\mod12$$
Second, if $p\equiv3\mod4$, $\left(\frac{-1}{p}\right)=-1$, then $\left(\frac{3}{p}\right)=-1$. And since $p\not\equiv3\mod4$, $\left(\frac{3}{p}\right)=-\left(\frac{p}{3}\right)=-1$, so $p\equiv1\mod3$, thus $$p\equiv7\mod12$$
In conclusion, $p\equiv1\mod6$, and since $p$ is odd prime, it can be deduced to $p\equiv1\mod3$.
\item Sufficiency: We know
$$p\equiv1\mod3$$
So we can get $$\left(\frac{p}{3}\right)=1$$
First, if $p\equiv1\mod4$, $$\left(\frac{-3}{p}\right)=\left(\frac{-1}{p}\right)\left(\frac{3}{p}\right)=1\cdot1=1$$
Second, if $p\equiv3\mod4$, $$\left(\frac{-3}{p}\right)=\left(\frac{-1}{p}\right)\cdot-\left(\frac{3}{p}\right)=-1\cdot-1=1$$
So it is proved.
\end{enumerate}
So $\left(\frac{-3}{p}\right)=1$ if and only if $p\equiv1\mod3$.

\item
Since $\left(\frac{a}{p}\right)=1$,
$$a^{(p-1)/2}\equiv1\mod p$$
And we know 2 is a prime factor of $p-1$, so it doesn't satisfy the condition that for all prime factors $q$ of $p-1$, $a^{(p-1)/q}\not\equiv1\mod p$. Then $a$ is not a generator of $F_p^*$.

\end{enumerate}

\section{Prime vs. irreducible}
\begin{enumerate}
\item
In an integral domain, suppose a prime element $p$ is reducible, so it can be implied as $p=ab$, where $a,b$ are non-zero, non-invertible and not equals to the ring element 1. Let $x=k_1a$, $y=k_2b$, $k_1,k_2\neq 0$, so $x,y\neq 0$. If $b\nmid k_1$ and $a\nmid k_2$, then $ab\nmid k_1a$ and $ab\nmid k_2b$, which means $p\nmid x$ and $p\nmid y$, which makes a contradiction with (*), so we can conclude that any prime element in an integral domain is reducible number is not prime. And since any number $p>1$ is either a prime or
\item
In $Z$, suppose an irreducible number $p>1$ is not prime, but it can't be implied as $p=ab$, where $a,b>1$. Suppose $a\mid p$, we can get $a=1$ or $a=p$, which makes a contradiction with (**). So we can conclude that any irreducible integer is prime in $Z$.
\item
From (**), we can simply get any prime number is irreducible. So if $p$ is a prime and $p\mid x\cdot y$, $x,y\in Z$, suppose $p\nmid x$ and $p\nmid y$, we can get $p\nmid x\cdot y$, which makes a contradiction. So we (*) is proved, and (**) implies (*).
\item
From (*), we know any prime integer is irreducible, if $p$ is a prime and $a|p$, suppose $a\neq1$ and $a\neq p$, then $1<a<p$, but $a|p$ and p is not reducible, which makes a contradiction, so (*) implies (**). And according to part 3, (**) implies (*), we can conclude that (*) and (**) are equivalent for integers.
\end{enumerate}


\section{Primitive root mod 65537}
\begin{enumerate}
\item
Since 65537 is a prime, we can calculate $3^{32768}\mod65537$ and we can find that $3^{32768}\equiv-1\mod65537$ (The calculation is shown in part 2), so $$\left(\frac{3}{65537}\right)=-1$$
\item
By applying modular exponentiation, we get the following table.
\begin{center}
\begin{tabular}{ccc}
$i$ & $d_i$ & power mod 65537 \\\hline
\input{ex5/2}
\end{tabular}
\end{center}

So $$3^{32768}\equiv65536\mod65537$$
$$3^{32768}\not\equiv-1\mod65537$$

\item
According to Theorem 2.17, we can conclude that 3 is a primitive root mod 65537 because 2 is the only prime factor of 65536 and $3^{(65537-1)/2}\not\equiv1\mod65537$.
\end{enumerate}

\end{document}
